Lang/OperationalSemantics.v
@@ -1,0 +1,34 @@
+Require Import Utf8.
+Require Import Syntax Semantics WeakHead.
+Require Import Binding.Lib Binding.Product Binding.Set.
+Require Import Relation_Operators.
+
+(* ========================================================================== *)
+(* Operational semantics of jumps *)
+
+Reserved Notation "J₁ ↦ⱼ J₂" (at level 50).
+
+Inductive jop {S : VSig} : jump S → jump S → Prop :=
+  | jop_beta : ∀ q E M (V : value S),
+    j_jmp q (eplug E (t_app (v_lam M) V)) ↦ⱼ j_jmp q (eplug E (subst M V))
+  | jop_ctrl : ∀ q E J,
+    j_jmp q (eplug E (t_ctrl J)) ↦ⱼ subst J (s_sub q E)
+
+where "J₁ ↦ⱼ J₂" := (@jop _ J₁ J₂).
+
+Notation jop_rtc J₁ J₂ := (clos_refl_trans _ jop J₁ J₂).
+Notation "J₁ '↦↦ⱼ' J₂" := (jop_rtc J₁ J₂) (at level 50).
+
+Lemma jop_jwh {S : VSig} (J₁ J₂ : jump S) :
+  J₁ ↦ⱼ  J₂ →
+  J₁ ↠ₕⱼ J₂.
+Proof.
+  intro Hop.
+  induction Hop.
+  - constructor. constructor.
+    induction E; term_simpl.
+    + constructor.
+    + constructor. apply IHE.
+    + constructor. apply IHE.
+  - apply jwh_ctrl_plug.
+Qed.
