Lang/WeakHead.v
@@ -1,0 +1,184 @@
+Require Import Utf8.
+Require Import Syntax Semantics.
+Require Import Binding.Lib Binding.Product Binding.Set.
+Require Import Relation_Operators.
+
+(* ========================================================================== *)
+(* Weak head reduction *)
+
+Reserved Notation "M₁ '→ₕₜ' M₂" (at level 50).
+Reserved Notation "J₁ '→ₕⱼ' J₂" (at level 50).
+
+Inductive twh {S : VSig} : term S → term S → Prop :=
+  | twh_beta : ∀ M (V : value S),
+    t_app (v_lam M) V →ₕₜ subst M V
+  | twh_C_L : ∀ (J : jump (incK S)) (N : term S),
+    t_app (t_ctrl J) N →ₕₜ t_ctrl (struct_subst J (e_appl e_hole (shift N)))
+  | twh_C_R : ∀ J (V : value S),
+    t_app V (t_ctrl J) →ₕₜ t_ctrl (struct_subst J (e_appr (shift V) e_hole))
+
+  | twh_app_L : ∀ M M' N,
+    M →ₕₜ M' →
+    t_app M N →ₕₜ t_app M' N
+  | twh_app_R : ∀ (V : value S) N N',
+    N →ₕₜ N' →
+    t_app V N →ₕₜ t_app V N'
+
+with jwh {S : VSig} : jump S → jump S → Prop :=
+  | jwh_C_idem : ∀ (q : katom S) (J : jump (incK S)),
+    j_jmp q (t_ctrl J) →ₕⱼ subst J (s_sub q e_hole)
+
+  | jwh_jmp : ∀ q M M',
+    M →ₕₜ M' →
+    j_jmp q M →ₕⱼ j_jmp q M'
+
+where "M₁ →ₕₜ M₂" := (@twh _ M₁ M₂)
+  and "J₁ →ₕⱼ J₂" := (@jwh _ J₁ J₂).
+
+Notation jwh_rtc J₁ J₂ := (clos_refl_trans _ jwh J₁ J₂).
+Notation "J₁ '↠ₕⱼ' J₂" := (jwh_rtc J₁ J₂) (at level 50).
+
+Notation twh_rtc M₁ M₂ := (clos_refl_trans _ twh M₁ M₂).
+Notation "M₁ '↠ₕₜ' M₂" := (twh_rtc M₁ M₂) (at level 50).
+
+(* -------------------------------------------------------------------------- *)
+
+Lemma twh_refl {S : VSig} (M : term S) :
+  M ↠ₕₜ M.
+Proof. constructor 2. Qed.
+Lemma jwh_refl {S : VSig} (J : jump S) :
+  J ↠ₕⱼ J.
+Proof. constructor 2. Qed.
+
+Lemma twh_app_L_cong {S : VSig} (M M' N : term S) :
+  M ↠ₕₜ M' →
+  t_app M N ↠ₕₜ t_app M' N.
+Proof. intro Hwh. cong Hwh. Qed.
+
+Lemma twh_app_R_cong {S : VSig} (V : value S) (N N' : term S) :
+  N ↠ₕₜ N' →
+  t_app V N ↠ₕₜ t_app V N'.
+Proof. intro Hwh. cong Hwh. Qed.
+
+Lemma jwh_jmp_cong {S : VSig} q (M M' : term S) :
+  M ↠ₕₜ M' →
+  j_jmp q M ↠ₕⱼ j_jmp q M'.
+Proof. intro Hwh. cong Hwh. Qed.
+
+Lemma twh_ctrl_plug {S : VSig} (J : jump (incK S)) E :
+  eplug E (t_ctrl J) ↠ₕₜ t_ctrl (struct_subst J (shift E)).
+Proof.
+  induction E.
+  + term_simpl. rewrite struct_subst_pure. apply twh_refl.
+  + term_simpl. econstructor 3.
+    { apply twh_app_L_cong.
+      apply IHE. }
+    econstructor 3.
+    { constructor. constructor. }
+    rewrite struct_subst_comp with (E₂ := e_appl e_hole M).
+    term_simpl. constructor 2.
+  + term_simpl. econstructor 3.
+    { apply twh_app_R_cong.
+      apply IHE. }
+    econstructor 3.
+    { constructor. constructor. }
+    rewrite struct_subst_comp with (E₂ := e_appr V e_hole).
+    term_simpl. constructor 2.
+Qed.
+
+Lemma jwh_ctrl_plug {S : VSig} q (J : jump (incK S)) E :
+  j_jmp q (eplug E (t_ctrl J)) ↠ₕⱼ subst J (s_sub q E).
+Proof.
+  econstructor 3.
+  { apply jwh_jmp_cong. apply twh_ctrl_plug. }
+  econstructor 3.
+  { constructor. constructor. }
+  rewrite subst_struct_subst. simpl.
+  constructor 2.
+Qed.
+
+(* -------------------------------------------------------------------------- *)
+(* alternative definition of jwh *)
+
+Inductive bcred {S : VSig} : term S → term S → Prop :=
+  | bcred_beta : ∀ M (V : value S),
+    bcred (t_app (v_lam M) V) (subst M V)
+  | bcred_C_L : ∀ (J : jump (incK S)) (N : term S),
+    bcred (t_app (t_ctrl J) N) (t_ctrl (struct_subst J (e_appl e_hole (shift N))))
+  | bcred_C_R : ∀ J (V : value S),
+    bcred (t_app V (t_ctrl J)) (t_ctrl (struct_subst J (e_appr (shift V) e_hole))).
+
+Notation "M₁ 'bcred*' M₂" := (clos_refl_trans _ bcred M₁ M₂) (at level 50).
+
+Reserved Notation "J₁ '→ₕⱼ'' J₂" (at level 50).
+
+Inductive jwh' {S : VSig} : jump S → jump S → Prop :=
+  | jwh_plug : ∀ q E M N,
+    bcred M N →
+    j_jmp q (eplug E M) →ₕⱼ' j_jmp q (eplug E N)
+  | jwh_idem : ∀ q J,
+    j_jmp q (t_ctrl J) →ₕⱼ' subst J (s_sub q e_hole)
+
+where "J₁ →ₕⱼ' J₂" := (@jwh' _ J₁ J₂).
+
+Notation jwh'_rtc J₁ J₂ := (clos_refl_trans _ jwh' J₁ J₂).
+Notation "J₁ '↠ₕⱼ'' J₂" := (jwh'_rtc J₁ J₂) (at level 50).
+
+Lemma twh_bcred {S : VSig} (M M' : term S) :
+  M →ₕₜ M' →
+  ∃ E N N',
+    M = eplug E N
+    ∧ M' = eplug E N'
+    ∧ bcred N N'.
+Proof.
+  intro Hwh.
+  induction Hwh.
+  - exists e_hole. repeat eexists. constructor.
+  - exists e_hole. repeat eexists. constructor.
+  - exists e_hole. repeat eexists. constructor.
+  - destruct IHHwh as [E [P [P' [? [? ?]]]]]. subst.
+    exists (e_appl E N). repeat eexists. assumption.
+  - destruct IHHwh as [E [P [P' [? [? ?]]]]]. subst.
+    exists (e_appr V E). repeat eexists. assumption.
+Qed.
+
+Lemma bcred_twh {S : VSig} E (M M' : term S) :
+  bcred M M' →
+  eplug E M →ₕₜ eplug E M'.
+Proof.
+  intro Hbcred.
+  induction E; term_simpl.
+  - destruct Hbcred; constructor.
+  - constructor. apply IHE.
+  - constructor. apply IHE.
+Qed.
+
+Lemma jwh_jwh' {S : VSig} (J J' : jump S) :
+  J →ₕⱼ  J' →
+  J →ₕⱼ' J'.
+Proof.
+  intro Hwh.
+  induction Hwh.
+  - constructor.
+  - apply twh_bcred in H.
+    destruct H as [E [N [N' [? [? ?]]]]]; subst.
+    constructor. apply H1.
+Qed.
+
+Lemma jwh'_jwh {S : VSig} (J J' : jump S) :
+  J →ₕⱼ' J' →
+  J →ₕⱼ  J'.
+Proof.
+  intro Hwh.
+  destruct Hwh.
+  - induction E; term_simpl.
+    + constructor. destruct H; constructor.
+    + constructor. constructor.
+      apply bcred_twh.
+      apply H.
+    + constructor. constructor.
+      apply bcred_twh.
+      apply H.
+  - constructor.
+Qed.
+
